Add x86

x86/Machregsaux.ml
@@ -10,6 +10,25 @@
 (*                                                                     *)
 (* *********************************************************************)
 
+open AST
+
 (** Auxiliary functions on machine registers *)
 
 let is_scratch_register r = false
+
+(* Function to get the target specific register class for AST types.
+   We have two main register classes:
+     0 for integer registers
+     1 for floating-point registers
+   plus a third pseudo-class 2 that has no registers and forces
+   stack allocation. *)
+
+let class_of_type = function
+  | Tint | Tlong -> 0
+  | Tfloat | Tsingle -> 1
+  | Tany32 -> 0
+  | Tany64 -> if Archi.ptr64 then 0 else 1
+
+let interferes_caller_save tv mr = not (Conventions1.is_callee_save mr)
+
+module AllocInterface = ArchitectureInterface.DefaultInterface
